icing/examples/dopplerProofsScript.sml
@@ -40,57 +40,111 @@ val plan_list = theAST_plan_result |> concl |> rhs (* Get the actual plan *)
 Theorem doppler_opts_icing_correct =
   mk_opt_correct_thm [Q.SPEC ‘FP_Add’ fp_comm_gen_correct, fp_fma_intro_correct];
 
-*)
-
 Theorem doppler_opts_real_id =
   mk_real_id_thm [SIMP_RULE (srw_ss()) [] (Q.SPEC ‘FP_Add’ fp_comm_gen_real_id), fma_intro_real_id];
 
+*)
+
 val st = get_ml_prog_state ();
 
-Definition doppler_real_spec_def:
-  doppler_real_spec (w1, w2, w3) = real_spec_prog ^body doppler_env ^fvars [w1;w2;w3]
-End
+val (args, argList, vList) =
+  if numArgs = 1 then (“(w1):word64”, “[w1]:word64 list”, “[d1]:v list”)
+  else if numArgs = 2 then (“(w1, w2):word64 # word64”, “[w1;w2]:word64 list”, “[d1; d2]:v list”)
+  else if numArgs = 3 then (“(w1, w2, w3):word64 # word64 # word64”,
+                            “[w1; w2; w3]:word64 list”,
+                            “[d1; d2; d3]:v list”)
+  else if numArgs = 4 then
+    (“(w1, w2, w3, w4):word64 # word64 # word64 #word64”,
+     “[w1; w2; w3; w4]:word64 list”,
+     “[d1; d2; d3; d4]:v list”)
+  else if numArgs = 6 then
+    (“(w1, w2, w3, w4, w5, w6):word64 # word64 # word64 # word64 # word64 #word64”,
+     “[w1; w2; w3; w4; w5; w6]:word64 list”,
+     “[d1; d2; d3; d4; d5; d6]:v list”)
+  else if numArgs = 8 then
+    (“(w1, w2, w3, w4, w5, w6, w7, w8):word64#word64#word64#word64#word64#word64#word64#word64”,
+     “[w1; w2; w3; w4; w5; w6; w7; w8]:word64 list”,
+     “[d1; d2; d3; d4; d5; d6; d7; d8]:v list”)
+  else (“(w1, w2, w3, w4, w5, w6, w7, w8, w9):word64#word64#word64#word64#word64#word64#word64#word64#word64”,
+        “[w1; w2; w3; w4; w5; w6; w7; w8; w9]:word64 list”,
+        “[d1; d2; d3; d4; d5; d6; d7; d8; d9]:v list”)
 
-Definition doppler_opt_float_option_noopt_def:
-  doppler_opt_float_option_noopt w1 w2 w3 =
-   case evaluate
-     (empty_state with fp_state := empty_state.fp_state with canOpt := FPScope NoOpt)
-   (doppler_env with v := extend_env_with_vars (REVERSE ^fvars) (REVERSE [w1;w2;w3]) (doppler_env).v)
-   [^body] of
+val theAST_real_spec_def =
+  Define ‘theAST_real_spec ^args = real_spec_prog ^body_opt theAST_env ^fvars ^argList’
+
+val theAST_opt_float_option_noopt_def =
+  Define ‘theAST_opt_float_option_noopt ^args =
+          case evaluate
+               (empty_state with fp_state := empty_state.fp_state with canOpt := FPScope NoOpt)
+               (theAST_env with v := extend_env_with_vars (REVERSE ^fvars) (REVERSE ^argList) (theAST_env).v)
+   [^body_opt] of
    | (st, Rval [FP_WordTree fp]) =>
      if st = (empty_state with fp_state := empty_state.fp_state with canOpt := FPScope NoOpt)
      then SOME fp else NONE
-   | _ => NONE
-End
+   | _ => NONE’
 
-Definition doppler_opt_float_option_def:
-  doppler_opt_float_option w1 w2 w3 =
-   case evaluate empty_state
-   (doppler_env with v := extend_env_with_vars (REVERSE ^fvars) (REVERSE [w1;w2;w3]) (doppler_env).v)
-   [^body] of
+val theAST_opt_float_option_def =
+  Define ‘theAST_opt_float_option ^args =
+         case evaluate empty_state
+                       (theAST_env with v := extend_env_with_vars (REVERSE ^fvars) (REVERSE ^argList) (theAST_env).v)
+   [^body_opt] of
    | (st, Rval [FP_WordTree fp]) => if (st = empty_state) then SOME fp else NONE
-   | _ => NONE
-End
+   | _ => NONE’
 
-Definition doppler_float_returns_def:
-  doppler_float_returns (w1,w2,w3) w ⇔
+val theAST_float_returns_def =
+  Define ‘
+  theAST_float_returns ^args w ⇔
   ∃ fpOpts st2 fp.
-   evaluate (empty_state with fp_state := empty_state.fp_state with <| rws := theOpts.optimisations ; opts := fpOpts; canOpt := FPScope NoOpt |>)
-   (doppler_env with v :=
-     extend_env_with_vars (REVERSE ^fvars) (REVERSE [w1;w2;w3]) (doppler_env).v)
-   [^body_before] = (st2, Rval [FP_WordTree fp]) ∧ compress_word fp = w
-End
+    let theOpts = FLAT (MAP (λ x. case x of |Apply (_, rws) => rws |_ => []) (HD theAST_plan)) in
+      evaluate (empty_state with fp_state :=
+                empty_state.fp_state with
+                           <| rws := theOpts ; opts := fpOpts; canOpt := FPScope NoOpt |>)
+               (theAST_env with v :=
+                extend_env_with_vars (REVERSE ^fvars) (REVERSE ^argList) (theAST_env).v)
+               [^body] = (st2, Rval [FP_WordTree fp]) ∧ compress_word fp = w’
 
-Theorem doppler_opt_backward_sim:
-  ∀ w1 w2 w3 w.
-  doppler_opt_float_option_noopt w1 w2 w3 = SOME w ⇒
-  doppler_float_returns (w1,w2,w3) (compress_word w)
+Theorem freeVars_list_body:
+  ∀ (st1:unit semanticPrimitives$state) st2.
+    freeVars_list_arithExp_bound
+      st1 st2 [^body]
+      (theAST_env with v :=
+       extend_env_with_vars (REVERSE ^fvars) (REVERSE ^argList) (theAST_env).v)
 Proof
-  simp[doppler_opt_float_option_noopt_def, doppler_float_returns_def]
+  rpt strip_tac
+  \\ gs[freeVars_arithExp_bound_def, icing_rewriterTheory.isFpArithExp_def,
+        freeVars_fp_bound_def]
+  \\ rpt conj_tac
+  (* Non-let goals are automatically solved *)
+  \\ TRY (gs[extend_env_with_vars_def] \\ NO_TAC)
+  (* Remainder: let-goals *)
+  \\ rpt strip_tac
+  (* Let-goals not reasoning about let-bound variable *)
+  \\ TRY (gs[extend_env_with_vars_def,namespaceTheory.nsOptBind_def] \\ NO_TAC)
+  \\ rveq
+  \\ qpat_x_assum ‘evaluate _ _ _ = _’ mp_tac
+  \\ qmatch_goalsub_abbrev_tac ‘evaluate theState theEnv [theExp] = _’
+  \\ ‘isFpArithExp theExp’ by (unabbrev_all_tac \\ EVAL_TAC)
+  \\ first_x_assum $ mp_then Any mp_tac (INST_TYPE [“:'a” |-> “:unit”] (CONJUNCT1 icing_rewriterProofsTheory.isFpArithExp_matched_evaluates))
+  \\ disch_then (qspecl_then [‘theEnv’, ‘theState’] mp_tac)
+  \\ impl_tac
+  (* free variables must be bound *)
+  \\ TRY (rpt strip_tac \\ rename1 ‘x IN FV theExp’ \\ unabbrev_all_tac
+          \\ gs[extend_env_with_vars_def, namespaceTheory.nsOptBind_def]
+          \\ NO_TAC)
+  (* use the theorem to prove the conclusion *)
+  \\ TRY (rpt strip_tac \\ imp_res_tac evaluatePropsTheory.evaluate_sing \\ gs[]
+          \\ rveq \\ gs[extend_env_with_vars_def, namespaceTheory.nsOptBind_def] \\ NO_TAC)
+QED
+
+Theorem theAST_opt_backward_sim:
+  theAST_opt_float_option_noopt ^args = SOME w ⇒
+  theAST_float_returns ^args (compress_word w)
+Proof
+  simp[theAST_opt_float_option_noopt_def, theAST_float_returns_def]
   \\ rpt gen_tac
   \\ ntac 5 (TOP_CASE_TAC \\ fs[])
   \\ strip_tac \\ rveq
-  \\ fs[GSYM local_opt_run_thm]
+  \\ fs[GSYM local_opt_thm]
   \\ first_x_assum (mp_then Any assume_tac no_optimisations_eval_sim)
   \\ fs[]
   \\ first_x_assum (qspecl_then [‘NoOpt’, ‘empty_state.fp_state.choices’] assume_tac)
@@ -100,61 +154,57 @@ Proof
   \\ fs[] \\ imp_res_tac noopt_sim_val \\ rveq
   \\ imp_res_tac noopt_sim_val_fp \\ rveq \\ fs[]
   \\ qpat_x_assum `evaluate _ _ _ = _` mp_tac
-  \\ qmatch_goalsub_abbrev_tac ‘evaluate emp_upd dEnv [optimise theOpts e_init] = (emp_res, _)’
+  \\ qmatch_goalsub_abbrev_tac ‘evaluate emp_upd dEnv [FST(optimise_with_plan theOpts thePlan e_init)] = (emp_res, _)’
   \\ strip_tac
-  \\ assume_tac (INST_TYPE [“:'a” |-> “:unit”] doppler_opts_icing_correct)
+  \\ assume_tac (INST_TYPE [“:'a” |-> “:unit”] stos_pass_correct_thm)
   \\ first_x_assum
        (qspecl_then [‘emp_upd’, ‘emp_res’, ‘dEnv’, ‘theOpts’, ‘[e_init]’, ‘[FP_WordTree fp2]’] mp_tac)
-  \\ simp[is_optimise_correct_def]
+  \\ simp[is_optimise_with_plan_correct_def]
   \\ impl_tac
   >- (
    unabbrev_all_tac
-   \\ fs[empty_state_def, theOpts_def, extend_conf_def, no_fp_opt_conf_def, doppler_env_def])
+   \\ fs[empty_state_def, theOpts_def, extend_conf_def, no_fp_opt_conf_def,
+         theAST_env_def, stos_pass_with_plans_def, theAST_plan_result]
+   \\ assume_tac freeVars_list_body \\ gs[theAST_env_def])
   \\ rpt strip_tac
   \\ unabbrev_all_tac
-  \\ fs[empty_state_def, semanticPrimitivesTheory.state_component_equality, doppler_env_def]
-  \\ pop_assum mp_tac
+  \\ fs[empty_state_def, semanticPrimitivesTheory.state_component_equality, theAST_env_def]
+  \\ qpat_x_assum ‘evaluate _ _ [ _ ] = _’ mp_tac
   \\ qmatch_goalsub_abbrev_tac ‘evaluate newSt newEnv _ = _’
   \\ strip_tac
   \\ qexists_tac ‘newSt.fp_state.opts’
   \\ unabbrev_all_tac
-  \\ first_x_assum (mp_then Any (qspec_then ‘0’ assume_tac) (CONJUNCT1 evaluate_add_choices))
+  \\ first_x_assum (mp_then Any (qspec_then ‘0’ assume_tac) (CONJUNCT1 fpSemPropsTheory.evaluate_add_choices))
   \\ fs[theOpts_def, no_fp_opt_conf_def, extend_conf_def,
-        config_component_equality]
+        config_component_equality, theAST_plan_result]
 QED
 
-val doppler_opt = theAST_opt |> concl |> rhs;
+val theAST_side_def =
+  Define ‘theAST_side ^args = (is_precond_sound ^fvars ^argList ^(theAST_pre_def |> concl |> rhs))’
 
-val theAST_pre = theAST_pre_def |> concl |> rhs;
-
-Definition doppler_side_def:
-  doppler_side w1 w2 w3 = (is_precond_sound ^fvars [w1; w2; w3] ^theAST_pre)
+Definition is_Double_def:
+  is_Double [] [] = T ∧
+  is_Double (w1::ws) (d1::ds) = (DOUBLE (Fp_const w1) d1 ∧ is_Double ws ds)
 End
 
-Definition doppler_real_fun_def:
-  doppler_real_fun w1 w2 w3 =
-    doppler_real_spec (w1,w2,w3)
-End
+val theAST_v = fetch_v (stringSyntax.fromHOLstring fname) st
+val theAST_v_def = DB.find ((term_to_string theAST_v)^"_def") |> hd |> #2 |> #1
 
-Theorem doppler_spec:
-  ∀ w1 w2 w3 d1 d2 d3.
-    doppler_side w1 w2 w3 ∧
-    DOUBLE (Fp_const w1) d1 ∧
-    DOUBLE (Fp_const w2) d2 ∧
-    DOUBLE (Fp_const w3) d3 ⇒
-    let result = (doppler_opt_float_option w1 w2 w3) in
-      (∀ p.
-        app (p:'ffi ffi_proj) ^(fetch_v "doppler" st)
-          [d1; d2; d3]
-          (emp)
-          (POSTv v.
-           &DOUBLE_RES result v)) ∧
-        doppler_float_returns (w1,w2,w3) (compress_word (THE result)) ∧
-      real$abs (fp64_to_real (compress_word (THE result)) - doppler_real_fun w1 w2 w3) ≤ theErrBound
+Theorem theAST_spec:
+  theAST_side ^args ∧
+  is_Double ^argList ^vList  ⇒
+  let result = (theAST_opt_float_option ^args) in
+    (∀ p.
+       app (p:'ffi ffi_proj) ^theAST_v
+           ^vList
+           (emp)
+           (POSTv v.
+            &DOUBLE_RES result v)) ∧
+    theAST_float_returns (w1,w2,w3) (compress_word (THE result)) ∧
+    real$abs (fp64_to_real (compress_word (THE result)) - theAST_real_spec ^args) ≤ theErrBound
 Proof
-  rpt gen_tac \\ simp[app_def, doppler_side_def]
+  rpt gen_tac \\ simp[app_def, theAST_side_def, is_Double_def]
   \\ rpt (disch_then assume_tac)
-  \\ simp[app_basic_def]
   \\ rpt (gen_tac ORELSE (disch_then assume_tac)) \\ fs[]
   \\ mp_tac errorbounds_AST
   \\ fs[isOkError_def, option_case_eq, pair_case_eq, getErrorbounds_def, stripFuns_def, PULL_EXISTS]
@@ -163,86 +213,125 @@ Proof
   \\ rpt (gen_tac ORELSE (disch_then assume_tac)) \\ fs[] \\ rveq
   \\ first_assum (mp_then Any mp_tac CakeML_FloVer_infer_error)
   \\ fs[checkErrorbounds_succeeds_def, PULL_EXISTS]
-  \\ qpat_x_assum ‘toFloVerCmd _ _ _ = SOME _’ mp_tac
-  \\ qmatch_goalsub_abbrev_tac ‘toFloVerCmd _ _ doppler_body = _’
-  \\ disch_then assume_tac
+  \\ qpat_x_assum ‘toFloVerCmd _ _ _ = SOME _’
+                  (fn th => disch_then (fn ith => mp_then Any mp_tac ith th) \\ assume_tac th)
+  \\ fs[theAST_pre_def]
   \\ disch_then (qspecl_then
-                 [‘doppler_env’,
-                  ‘Fun "u" (Fun "v" (Fun "t" doppler_body))’] mp_tac)
-  \\ unabbrev_all_tac
-  \\ fs[stripFuns_def, theAST_pre_def]
+                 [‘theAST_env’,
+                  ‘case ^(theAST_opt |> concl |> rhs) of | [Dlet _ _ e] => e’] mp_tac)
+  \\ impl_tac
+  >- fs[stripFuns_def]
   \\ strip_tac
-  \\ simp[semanticPrimitivesTheory.do_opapp_def, doppler_v_def]
+  \\ simp[semanticPrimitivesTheory.do_opapp_def, theAST_v_def]
   \\ reverse conj_tac
   >- (
    rpt (pop_assum mp_tac) \\ simp[] \\ rpt (disch_then assume_tac)
    \\ rveq
-   \\ ‘doppler_opt_float_option_noopt w1 w2 w3 = SOME fp’
-      by (fs[doppler_opt_float_option_noopt_def])
-   \\ imp_res_tac doppler_opt_backward_sim
-   \\ rfs[doppler_opt_float_option_def, doppler_real_fun_def,
-          real_spec_prog_def, doppler_real_spec_def]
-   \\ assume_tac (INST_TYPE [“:'a” |-> “:unit”] doppler_opts_real_id)
+   \\ ‘theAST_opt_float_option_noopt ^args = SOME fp’
+      by (fs[theAST_opt_float_option_noopt_def])
+   \\ imp_res_tac theAST_opt_backward_sim
+   \\ rfs[theAST_opt_float_option_def, theAST_real_spec_def,
+          real_spec_prog_def, theAST_real_spec_def]
+   \\ assume_tac (INST_TYPE [“:'a” |-> “:unit”] stos_pass_real_id_thm)
    \\ qpat_x_assum `evaluate _ _ [realify _] = _` mp_tac
    \\ unabbrev_all_tac
-   \\ simp[GSYM local_opt_run_thm]
-   \\ qmatch_goalsub_abbrev_tac ‘evaluate _ _ [realify (no_optimisations theOpts e_opt)] = _’
+   \\ simp[GSYM local_opt_thm]
+   \\ qmatch_goalsub_abbrev_tac ‘evaluate _ _ [realify (no_optimisations theOpts (FST e_opt))] = _’
    \\ disch_then (mp_then Any mp_tac evaluate_no_optimisations)
    \\ fs[]
    \\ disch_then (qspecl_then [‘NoOpt’, ‘empty_state.fp_state.choices’] mp_tac)
    \\ impl_tac \\ unabbrev_all_tac
    >- (EVAL_TAC)
-   \\ qmatch_goalsub_abbrev_tac ‘evaluate emptyWithReals realEnv [realify (optimise theOpts e_init)] = _’
+   \\ qmatch_goalsub_abbrev_tac ‘evaluate emptyWithReals realEnv [realify (FST (optimise_with_plan theOpts thePlan e_init))] = _’
    \\ strip_tac
-   \\ fs[is_real_id_optimise_def]
+   \\ fs[is_real_id_optimise_with_plan_def]
    \\ first_x_assum (
       qspecl_then [ ‘emptyWithReals’, ‘emptyWithReals’, ‘realEnv’, ‘theOpts’, ‘[e_init]’, ‘[Real r]’] mp_tac)
    \\ simp[MAP]
-   \\ ‘theOpts with optimisations := [fp_comm_gen FP_Add; fp_fma_intro] = theOpts’
-      by (simp[theOpts_def, extend_conf_def, no_fp_opt_conf_def])
-   \\ pop_assum (fs o single)
-   \\ unabbrev_all_tac \\ fs[theOpts_def, no_fp_opt_conf_def]
-   \\ rpt strip_tac \\ rveq
-   \\ imp_res_tac evaluate_realify_state
-   \\ pop_assum mp_tac \\ impl_tac >- EVAL_TAC
+   \\ unabbrev_all_tac \\ fs[theAST_plan_result]
+   \\ impl_tac
+   >- (
+    imp_res_tac evaluate_realify_state
+    \\ qpat_x_assum `isPureExp _ ⇒ _ = _` mp_tac
+    \\ impl_tac >- EVAL_TAC
+    \\ strip_tac \\ fs[theOpts_def, no_fp_opt_conf_def])
    \\ strip_tac \\ rveq
-   \\ fs[empty_state_def, semanticPrimitivesTheory.fpState_component_equality, semanticPrimitivesTheory.state_component_equality]
    \\ irule REAL_LE_TRANS \\ asm_exists_tac \\ fs[])
+  \\ ntac (numArgs-1)
+          (rpt strip_tac \\ once_rewrite_tac [app_basic_def]
+           \\ simp[semanticPrimitivesTheory.do_opapp_def, set_sepTheory.cond_def]
+           \\ rpt strip_tac
+           (* We will return a val but we do not know which one *)
+           \\ Q.REFINE_EXISTS_TAC ‘Val v’
+           \\ simp[evaluate_to_heap_def, evaluate_ck_def, terminationTheory.evaluate_def]
+           \\ ntac 2 (qexists_tac ‘EMPTY’)
+           \\ fs[emp_def, set_sepTheory.SPLIT_def, cfHeapsBaseTheory.SPLIT3_def,
+                 set_sepTheory.SEP_EXISTS]
+           \\ simp[Once set_sepTheory.STAR_def]
+           \\ qexists_tac ‘emp’
+           \\ rpt (qexists_tac ‘EMPTY’) \\ conj_tac
+           >- fs[emp_def, set_sepTheory.SPLIT_def, cfHeapsBaseTheory.SPLIT3_def]
+           \\ conj_tac
+           >- fs[emp_def])
+  \\ once_rewrite_tac [app_basic_def]
+  \\ simp[semanticPrimitivesTheory.do_opapp_def, set_sepTheory.cond_def]
   \\ rpt strip_tac
   \\ Q.REFINE_EXISTS_TAC ‘Val v’
-  \\ simp[evaluate_to_heap_def, evaluate_ck_def, terminationTheory.evaluate_def]
-  \\ qexists_tac ‘EMPTY’ \\ qexists_tac ‘EMPTY’
-  \\ fs[emp_def, set_sepTheory.SPLIT_def, cfHeapsBaseTheory.SPLIT3_def]
-  \\ simp[set_sepTheory.SEP_EXISTS]
-  \\ qexists_tac ‘emp’ \\ simp[set_sepTheory.STAR_def]
-  \\ ntac 2 (qexists_tac ‘EMPTY’)
-  \\ fs[emp_def, set_sepTheory.SPLIT_def, cfHeapsBaseTheory.SPLIT3_def]
-  \\ simp[set_sepTheory.cond_def]
-  \\ rpt strip_tac
-  \\ Q.REFINE_EXISTS_TAC ‘Val v’ \\ simp[]
-  \\ ntac 2 (qexists_tac ‘EMPTY’) \\ rpt conj_tac \\ TRY (simp[DISJOINT_DEF] \\ NO_TAC)
-  \\ qexists_tac ‘emp’ \\ simp[emp_def]
-  \\ rpt strip_tac
-  \\ Q.REFINE_EXISTS_TAC ‘Val v’ \\ simp[]
-  \\ ‘DISJOINT (st2heap p st'') EMPTY’ by (simp[DISJOINT_DEF])
-  \\ asm_exists_tac \\ simp[DOUBLE_RES_def]
-  \\ rveq \\ simp[doppler_opt_float_option_def]
-  \\ first_x_assum (mp_then Any mp_tac (INST_TYPE [“:'a”|->“:unit”, “:'b”|->“:'ffi”] isPureExpList_swap_state))
-  \\ disch_then (qspec_then ‘st'' with clock := 0’ mp_tac)
+  \\ simp[DOUBLE_RES_def, theAST_opt_float_option_def]
+  \\ fs[emp_def] \\ rveq
+  \\ qexists_tac ‘EMPTY’
+  \\ rename1 ‘st2heap p st_final’
+  \\ qexists_tac ‘st2heap p st_final’ \\ conj_tac
+  >- fs[emp_def, set_sepTheory.SPLIT_def, cfHeapsBaseTheory.SPLIT3_def]
+  \\ simp[evaluate_to_heap_def, evaluate_ck_def]
+  \\ first_x_assum
+     (mp_then Any mp_tac
+      (INST_TYPE [“:'a”|->“:unit”, “:'b”|->“:'ffi”] pureExpsTheory.isPureExpList_swap_state))
+  \\ disch_then (qspec_then ‘st_final with clock := 0’ mp_tac)
   \\ impl_tac \\ fs[]
   >- (unabbrev_all_tac \\ EVAL_TAC)
-  \\ strip_tac \\ qexists_tac ‘0’ \\ fs[extend_env_with_vars_def, DOUBLE_def, doppler_env_def]
+  \\ strip_tac \\ qexists_tac ‘0’ \\ fs[extend_env_with_vars_def, DOUBLE_def, theAST_env_def]
 QED
+
+val (cl_list, inp_list, inps) =
+  let val (cstStrs, inps) =
+      if numArgs = 1 then
+        (“[cst1s]:mlstring list”, “(cst1s):mlstring”)
+      else if numArgs = 2 then
+        (“[cst1s; cst2s]:mlstring list”, “(cst1s,cst2s):mlstring#mlstring”)
+      else if numArgs = 3 then
+        (“[cst1s; cst2s; cst3s]:mlstring list”,
+        “(cst1s, cst2s, cst3s):mlstring#mlstring#mlstring”)
+      else if numArgs = 4 then
+        (“[cst1s; cst2s; cst3s; cst4s]:mlstring list”,
+        “(cst1s, cst2s, cst3s, cst4s):mlstring#mlstring#mlstring#mlstring”)
+      else if numArgs = 6 then
+        (“[cst1s; cst2s; cst3s; cst4s; cst5s; cst6s]:mlstring list”,
+        “(cst1s, cst2s, cst3s, cst4s, cst5s, cst6s):
+          mlstring#mlstring#mlstring#mlstring#mlstring#mlstring”)
+      else if numArgs = 8 then
+        (“[cst1s; cst2s; cst3s; cst4s; cst5s; cst6s; cst7s; cst8s]:mlstring list”,
+        “(cst1s, cst2s, cst3s, cst4s, cst5s, cst6s, cst7s, cst8s):
+          mlstring#mlstring#mlstring#mlstring#mlstring#mlstring#mlstring#mlstring”)
+      else (* numArgs = 9 *)
+        (“[cst1s; cst2s; cst3s; cst4s; cst5s; cst6s; cst7s; cst8s; cst9s]:mlstring list”,
+        “(cst1s, cst2s, cst3s, cst4s, cst5s, cst6s, cst7s, cst8s, cst9s):
+          mlstring#mlstring#mlstring#mlstring#mlstring#mlstring#mlstring#mlstring#mlstring”)
+  in (EVAL (Parse.Term ‘[fname] ++ ^cstStrs’) |> concl |> rhs, cstStrs, inps)
+  end
+
+Definition all_float_string_def:
+  all_float_string [] [] = T ∧
+  all_float_string (s1::ss) (w1::ws) = (is_float_string s1 w1 ∧ all_float_string ss ws)
+End
 
 Theorem main_spec:
   ∀ p.
-  cl = [fname; cst1s; cst2s; cst3s] ∧
-  is_float_string cst1s c1 ∧
-  is_float_string cst2s c2 ∧
-  is_float_string cst3s c3 ∧
-  doppler_side c1 c2 c3 ⇒
+  cl = ^cl_list ∧
+  all_float_string ^inp_list ^argList ∧
+  theAST_side ^args ⇒
   let
-    result = doppler_opt_float_option c1 c2 c3
+    result = theAST_opt_float_option ^args
   in
   app p ^(fetch_v "main" st)
     [Conv NONE []]
@@ -250,34 +339,37 @@ Theorem main_spec:
     (POSTv uv. &UNIT_TYPE () uv *
      STDIO (add_stdout fs (mlint$toString (&w2n (compress_word (THE result))))))
     ∧
-    doppler_float_returns (c1,c2,c3) (compress_word (THE result)) ∧
+    theAST_float_returns ^args (compress_word (THE result)) ∧
     real$abs (fp64_to_real (compress_word (THE result)) -
-      doppler_real_fun c1 c2 c3) ≤ theErrBound
+      theAST_real_spec ^args) ≤ theErrBound
 Proof
-  simp[] \\ rpt strip_tac
-  \\ first_x_assum (mp_then Any assume_tac (SIMP_RULE std_ss [] (INST_TYPE [“:'ffi”|->“:'a”] doppler_spec)))
+  simp[all_float_string_def] \\ rpt strip_tac
+  \\ first_x_assum $ mp_then Any assume_tac
+                   $ SIMP_RULE std_ss [is_Double_def] (INST_TYPE [“:'ffi”|->“:'a”] theAST_spec)
   >- (
    xcf "main" st
+   (* let for unit value *)
    \\ xlet_auto >- (xcon \\ xsimpl)
-   \\ ‘4 = LENGTH cl’ by (rveq \\ fs[])
+   \\ ‘^(numSyntax.term_of_int (numArgs+1)) = LENGTH cl’ by (rveq \\ fs[])
    \\ rveq
-   \\ xlet_auto_spec (SOME reader3_spec)
+   \\ xlet_auto_spec (SOME reader_spec)
    >- (xsimpl \\ qexists_tac ‘emp’ \\ xsimpl
        \\ qexists_tac ‘fs’ \\ xsimpl)
    \\ xmatch
    \\ fs[PAIR_TYPE_def] \\ reverse conj_tac
    >- (EVAL_TAC \\ fs[])
-   \\ rveq \\ fs[is_float_string_def]
-   \\ xlet_auto_spec (SOME intToFP_spec)
-   >- (xsimpl \\ qexists_tac ‘emp’ \\ xsimpl
-       \\ qexists_tac ‘fs’ \\ xsimpl)
-   \\ xlet ‘POSTv uv. &(DOUBLE (Fp_const ((n2w (Num i')):word64)) uv) * STDIO fs’
-   >- (xapp \\ xsimpl \\ asm_exists_tac \\ fs[])
-   \\ xlet ‘POSTv uv. &(DOUBLE (Fp_const ((n2w (Num i'')):word64)) uv) * STDIO fs’
-   >- (xapp \\ xsimpl \\ asm_exists_tac \\ fs[])
-   \\ rveq
-   \\ first_x_assum (qspecl_then [‘uv'’, ‘uv''’, ‘uv'3'’] mp_tac)
-   \\ impl_tac \\ fs[] \\ strip_tac
+   \\ rveq \\ fs[is_float_string_def] \\ rveq
+   \\ ntac numArgs (
+     last_x_assum (mp_then Any mp_tac intToFP_spec)
+     \\ disch_then (fn ith => last_x_assum $ mp_then Any mp_tac ith)
+     \\ disch_then drule
+     \\ disch_then (qspecl_then [‘p’, ‘fs’] assume_tac)
+     \\ xlet_auto
+     >- (xsimpl \\ qexists_tac ‘emp’ \\ xsimpl
+         \\ qexists_tac ‘fs’ \\ xsimpl)
+     \\ qpat_x_assum `app _ intToFP_v _ _ _` kall_tac)
+   \\ first_x_assum drule
+   \\ rpt (disch_then drule) \\ strip_tac
    \\ xlet_auto >- xsimpl
    \\ qpat_x_assum ‘DOUBLE_RES _ _’ mp_tac
    \\ simp[DOUBLE_RES_def] \\ TOP_CASE_TAC \\ fs[]
@@ -312,19 +404,17 @@ Proof
 QED
 
 Theorem main_whole_prog_spec:
-  cl = [fname; cst1s; cst2s; cst3s] ∧
-  is_float_string cst1s c1 ∧
-  is_float_string cst2s c2 ∧
-  is_float_string cst3s c3 ∧
-  doppler_side c1 c2 c3 ⇒
+  cl = ^cl_list ∧
+  all_float_string ^inp_list ^argList ∧
+  theAST_side ^args ⇒
   whole_prog_spec ^(fetch_v "main" st) cl fs
   NONE
   ((=)
-   (add_stdout fs (mlint$toString (&w2n (compress_word (THE (doppler_opt_float_option c1 c2 c3)))))))
+   (add_stdout fs (mlint$toString (&w2n (compress_word (THE (theAST_opt_float_option ^args)))))))
   ∧
-  doppler_float_returns (c1,c2,c3) (compress_word (THE (doppler_opt_float_option c1 c2 c3))) ∧
-  real$abs (fp64_to_real (compress_word (THE (doppler_opt_float_option c1 c2 c3))) -
-            doppler_real_fun c1 c2 c3) ≤ theErrBound
+  theAST_float_returns ^args (compress_word (THE (theAST_opt_float_option ^args))) ∧
+  real$abs (fp64_to_real (compress_word (THE (theAST_opt_float_option ^args))) -
+            theAST_real_spec ^args) ≤ theErrBound
 Proof
   simp[whole_prog_spec_def]
   \\ qmatch_goalsub_abbrev_tac`fs1 = _ with numchars := _`
@@ -343,55 +433,40 @@ val name = "main";
 
 val (prog_rewrite, semantics_prog_thm) = mk_whole_prog_spec_thm spec name (get_ml_prog_state());
 
-val doppler_prog_tm = rhs (concl prog_rewrite);
+val theAST_prog_tm = rhs (concl prog_rewrite);
 
-val doppler_prog_def = Define`doppler_prog = ^doppler_prog_tm`;
+val theAST_prog_def = Define`theAST_prog = ^theAST_prog_tm`;
 
 val full_semantics_prog_thm =
-  LIST_CONJ [
-    DISCH_ALL semantics_prog_thm,
-    CONJUNCT2 (SIMP_RULE std_ss [cfSupportTheory.IMP_SPLIT] main_whole_prog_spec)
-              |> SIMP_RULE std_ss [GSYM cfSupportTheory.IMP_SPLIT]
-              |> REWRITE_RULE [CONJ_ASSOC]
-              |> ONCE_REWRITE_RULE [CONJ_COMM]
-              |> ONCE_REWRITE_RULE [GSYM AND_IMP_INTRO]
-              |> ONCE_REWRITE_RULE [CONJ_COMM]
-              |> ONCE_REWRITE_RULE [GSYM AND_IMP_INTRO]
-              |> ONCE_REWRITE_RULE [CONJ_COMM]
-              |> ONCE_REWRITE_RULE [GSYM AND_IMP_INTRO]
-              |> ONCE_REWRITE_RULE [CONJ_COMM]
-              |> ONCE_REWRITE_RULE [GSYM AND_IMP_INTRO]
-  ]
-  |> SIMP_RULE std_ss [GSYM AND_IMP_INTRO]
-  |> SIMP_RULE std_ss [GSYM cfSupportTheory.IMP_SPLIT];
+      CONJUNCT2 (SIMP_RULE std_ss [cfSupportTheory.IMP_SPLIT] main_whole_prog_spec)
+              |> SIMP_RULE std_ss [GSYM cfSupportTheory.IMP_SPLIT, GSYM AND_IMP_INTRO]
+              |> UNDISCH_ALL
+              |> (fn th => LIST_CONJ [semantics_prog_thm, th])
+              |> DISCH_ALL |> SIMP_RULE std_ss [];
 
-Theorem doppler_semantics =
-  full_semantics_prog_thm |> ONCE_REWRITE_RULE[GSYM doppler_prog_def]
+Theorem theAST_semantics =
+  full_semantics_prog_thm |> ONCE_REWRITE_RULE[GSYM theAST_prog_def]
   |> DISCH_ALL |> SIMP_RULE std_ss [AND_IMP_INTRO,GSYM CONJ_ASSOC];
 
-Definition doppler_semantics_side_def:
-  doppler_semantics_side (s1,s2,s3) (c1,c2,c3) ⇔
-    is_float_string s1 c1 ∧
-    is_float_string s2 c2 ∧
-    is_float_string s3 c3 ∧
-    doppler_side c1 c2 c3
+Definition theAST_semantics_side_def:
+  theAST_semantics_side ^inps ^args ⇔
+    all_float_string ^inp_list ^argList ∧
+    theAST_side ^args
 End
 
-Theorem doppler_semantics_final:
-  doppler_semantics_side (s1,s2,s3) (c1,c2,c3) ∧ init_ok ([fname;s1;s2;s3],fs) ⇒
+Theorem theAST_semantics_final:
+  theAST_semantics_side ^inps ^args ∧ init_ok (^cl_list,fs) ⇒
   ∃ (w:word64).
-    CakeML_evaluates_and_prints ([fname;s1;s2;s3],fs,doppler_prog) (toString w) ∧
-    doppler_float_returns (c1,c2,c3) w ∧
-    real$abs (fp64_to_real w - doppler_real_fun c1 c2 c3) ≤ theErrBound
+    CakeML_evaluates_and_prints (^cl_list,fs,theAST_prog) (toString w) ∧
+    theAST_float_returns ^args w ∧
+    real$abs (fp64_to_real w - theAST_real_spec ^args) ≤ theErrBound
 Proof
   rpt strip_tac
-  \\ fs[init_ok_def, CakeML_evaluates_and_prints_def, doppler_semantics_side_def]
-  \\ first_x_assum (mp_then Any mp_tac doppler_semantics)
-  \\ rpt (disch_then drule)
-  \\ strip_tac \\ fs[]
-  \\ first_x_assum (qspecl_then [‘fs’,‘fname’] mp_tac)
-  \\ strip_tac \\ rfs[]
-  \\ qexists_tac ‘compress_word (THE (doppler_opt_float_option c1 c2 c3))’ \\ fs[]
+  \\ fs[init_ok_def, CakeML_evaluates_and_prints_def, theAST_semantics_side_def]
+  \\ first_x_assum (mp_then Any mp_tac theAST_semantics)
+  \\ rpt (disch_then drule) \\ fs[]
+  \\ disch_then drule \\ strip_tac
+  \\ qexists_tac ‘compress_word (THE (theAST_opt_float_option ^args))’ \\ fs[]
   \\ asm_exists_tac \\ fs[toString_def]
 QED
 
